
ax + by = c
dx + ey = f

ae
ce
db
fb

(a - d)x + (b - e)y = c - f
(a - d)x = c - f + (b - e)y

ax - dx = c - f + by - ey


=> x = c - f + (b - e)y / (a - d)
x = -1 - 7 + (3 - 1)y / 1 - 4
x = -8 + 2y / -3

(b - e)y = (c - f) - (a - d)x

=> y = (c - f) - (a - d)x / (b - e)

y = (-1 - 7) - (1 - 4)x / (3 - 1)
y = -8 + 3x / 2


x = [-8 + 2((-8 + 3x) / 2)] / -3


=> x, y 출력

// a, b, c, d, e, f 차례대로 입력
x + 3y = -1 => ax + by = e
4x + y = 7 => cx + dy = f

===
int x = (ce - bf) / (ae - bd);
int y = (cd - af) / (bd - ae);



a b c d e f
1 3 -1 4 1 7

a, d => a != d && (a > d || d > a), a * d or d * a
b, e

|a - d| < |b - e| or |a - d| > |b - e|

a * d
x = 1, 4
y = 3, 1
우항 = -1, 7

x1 * y1 - x2 * y2 = -1
x1 * y2 + x2 * y1 = 12













